Superposition_Calculus/Renaming.thy
@@ -11,6 +11,7 @@ locale renaming =
   assumes infinite_variables: "infinite variables"
 begin
 
+
 (* TODO: generalize? *)
 lemma renaming_exists: 
   assumes
